Add a total compiler in source_eval
Add a hook where an additional compiler can be provided and
used to invent "dummy" data to extend an oracle to infinity.
Unlike the standard compiler, this additional compiler must be
total. Prove that the generated oracle is well-formed in that
every step is taken by one of the two compilers.

compiler/backend/proofs/source_evalProofScript.sml
@@ -1,17 +1,15 @@
 (*
-  Proofs that the source_eval attachment of the compiler
-  preserves semantics, and that the oracle semantics can
-  be introduced
+  Proofs that the eval mode of the source semantics can
+  be switched to one that includes an oracle.
 *)
 
 open preamble semanticsTheory namespacePropsTheory
      semanticPrimitivesTheory semanticPrimitivesPropsTheory
-     source_evalTheory evaluatePropsTheory evaluateTheory
-     experimentalLib
+     evaluatePropsTheory evaluateTheory experimentalLib
 
 val _ = new_theory "source_evalProof";
 
-val _ = set_grammar_ancestry ["ast", "source_eval", "string",
+val _ = set_grammar_ancestry ["ast", "string",
     "semantics", "semanticPrimitivesProps"];
 
 (* an instance of custom_do_eval that behaves as much as possible
@@ -94,9 +92,10 @@ Proof
 QED
 
 Theorem env_rel_nsLift:
-  env_rel R (env with <| v := v |>) (env' with <| v := v' |>) ==>
-  env_rel R (env with <| v := nsLift mn v |>)
-    (env' with <| v := nsLift mn v' |>)
+  env_rel R (env with <| v := v; c := c |>)
+    (env' with <| v := v'; c := c' |>) ==>
+  env_rel R (env with <| v := nsLift mn v; c := nsLift mn c |>)
+    (env' with <| v := nsLift mn v'; c := nsLift mn c' |>)
 Proof
   rw [] \\ fs [env_rel_def, nsDom_nsLift, nsDomMod_nsLift]
   \\ rw [namespacePropsTheory.nsLookup_nsLift]
@@ -143,6 +142,13 @@ Proof
   \\ fs [Q.ISPEC `nsDom ns` EXTENSION, nsLookup_nsDom]
   \\ res_tac
   \\ fs []
+QED
+
+Triviality env_rel_nsLookup_c:
+  env_rel R env env' /\ nsLookup env.c id = r ==>
+  env'.c = env.c
+Proof
+  rw [env_rel_def]
 QED
 
 
@@ -206,18 +212,32 @@ QED
 
 val _ = bossLib.augment_srw_ss [rewrites [v_rel_l_simps, v_rel_Boolv]];
 
+Definition recorded_orac_wf_def:
+  recorded_orac_wf (compiler : compiler_fun) (orac : eval_oracle_fun) <=>
+  (0 < FST (FST (orac 0)) ==>
+    ?r. compiler (orac (FST (FST (orac 0)))) = SOME r /\
+        FST r (FST (SND (orac 0)))) /\
+  (!j. j < FST (FST (orac 0)) /\ 0 < j ==>
+    ?r. compiler (orac j) = SOME r /\ FST r (FST (SND (orac (j + 1)))))
+End
+
 Definition s_rel_def:
-  s_rel s s' <=>
-  ? dec_s orac_s init_s refs'. s' = s with <| refs := refs';
+  s_rel init_eds s s' <=>
+  ? dec_s orac_s refs'. s' = s with <| refs := refs';
     eval_state := SOME (EvalOracle orac_s) |> /\
   LIST_REL (sv_rel (v_rel orac_s)) s.refs refs' /\
   s.eval_state = SOME (EvalDecs dec_s) /\
-  orac_s.custom_do_eval = do_eval_record dec_s.compiler init_s /\
+  orac_s.custom_do_eval = do_eval_record init_eds.compiler
+    init_eds.compiler_state /\
   dec_s.compiler_state = (if FST (FST (orac_s.oracle 0)) = 0
-    then init_s else ((=) (FST (SND (orac_s.oracle 0))))) /\
+    then init_eds.compiler_state else ((=) (FST (SND (orac_s.oracle 0))))) /\
+  (0 < FST (FST (orac_s.oracle 0)) ==>
+    init_eds.compiler_state (FST (SND (orac_s.oracle 1)))) /\
   dec_s.env_id_counter = (orac_s.generation,
         LENGTH (EL orac_s.generation orac_s.envs), LENGTH orac_s.envs) /\
-  orac_s.generation < LENGTH orac_s.envs
+  orac_s.generation < LENGTH orac_s.envs /\
+  dec_s.compiler = init_eds.compiler /\
+  recorded_orac_wf init_eds.compiler orac_s.oracle
 End
 
 Definition orac_s_def:
@@ -314,7 +334,7 @@ Proof
 QED
 
 Theorem s_rel_store_lookup:
-  s_rel s t /\ j = i /\ es = orac_s t.eval_state ==>
+  s_rel init_eds s t /\ j = i /\ es = orac_s t.eval_state ==>
   OPTREL (sv_rel (v_rel es)) (store_lookup i s.refs) (store_lookup j t.refs)
 Proof
   rw [s_rel_def]
@@ -342,7 +362,7 @@ Proof
 QED
 
 Theorem pmatch:
-  s_rel s t /\ es = orac_s t.eval_state /\ env_rel (v_rel es) env env' ==>
+  s_rel init_eds s t /\ es = orac_s t.eval_state /\ env_rel (v_rel es) env env' ==>
   (!env_c s_refs p x binds y binds'.
   s_refs = s.refs /\ env_c = env.c /\
   v_rel es x y /\
@@ -363,7 +383,7 @@ Proof
   disch_tac
   \\ ho_match_mp_tac terminationTheory.pmatch_ind
   \\ rw [terminationTheory.pmatch_def, match_result_rel_def,
-    quotient_pairTheory.PAIR_REL_THM, compile_pat_def]
+    quotient_pairTheory.PAIR_REL_THM]
   \\ rveq \\ fs []
   \\ imp_res_tac v_to_env_id_SOME
   \\ fs [terminationTheory.pmatch_def]
@@ -394,14 +414,22 @@ Proof
   )
 QED
 
-Triviality pmatch_use = UNDISCH_ALL pmatch |> CONJUNCT1 |> SPEC_ALL
-  |> Q.INST [`binds` |-> `[]`]
-  |> DISCH_ALL |> GEN_ALL
-  |> SIMP_RULE list_ss []
+Triviality pmatch_drule_form:
+  pmatch env.c s.refs p x [] = res ∧
+  s_rel init_eds s t ∧ env_rel (v_rel (orac_s t.eval_state)) env env' ∧
+  v_rel (orac_s t.eval_state) x y ⇒
+  match_result_rel T (LIST_REL ($= ### v_rel (orac_s t.eval_state)))
+    res (pmatch env'.c t.refs p y [])
+Proof
+  rw []
+  \\ irule (UNDISCH_ALL pmatch |> CONJUNCT1 |> DISCH_ALL)
+  \\ simp []
+  \\ metis_tac []
+QED
 
 Theorem can_pmatch_all:
   can_pmatch_all env.c s.refs pats x /\
-  s_rel s t /\
+  s_rel init_eds s t /\
   env_rel (v_rel (orac_s t.eval_state)) env env' /\
   v_rel (orac_s t.eval_state) x y ==>
   can_pmatch_all env'.c t.refs pats y
@@ -409,7 +437,7 @@ Proof
   rw []
   \\ Induct_on `pats`
   \\ rw [can_pmatch_all_def]
-  \\ drule pmatch_use
+  \\ drule (pmatch_drule_form |> GEN_ALL |> SIMP_RULE bool_ss [])
   \\ rpt (disch_then drule)
   \\ disch_then (qspec_then `h` mp_tac)
   \\ simp [match_result_rel_def]
@@ -534,9 +562,9 @@ Theorem sv_rel_l_cases =
   |> map (SIMP_CONV (srw_ss ()) [sv_rel_cases])
   |> map GEN_ALL |> LIST_CONJ
 
-Theorem do_app:
+Theorem do_app_sim:
   do_app (s.refs, s.ffi) op (REVERSE xs) = SOME ((refs, ffi), r) /\
-  s_rel s t /\
+  s_rel init_eds s t /\
   LIST_REL (v_rel (orac_s t.eval_state)) xs ys /\
   r <> Rerr (Rabort Rtype_error)
   ==>
@@ -584,13 +612,12 @@ Proof
 QED
 
 Theorem s_rel_clock:
-  s_rel s t ==> s.clock = t.clock /\
-    s_rel (dec_clock s) (dec_clock t)
+  s_rel init_eds s t ==> s.clock = t.clock /\
+    s_rel init_eds (dec_clock s) (dec_clock t)
 Proof
   rw [s_rel_def]
   \\ fs [evaluateTheory.dec_clock_def]
   \\ simp [semanticPrimitivesTheory.state_component_equality]
-  \\ qexists_tac `init_s`
   \\ simp []
 QED
 
@@ -826,21 +853,37 @@ Proof
   \\ imp_res_tac v_to_word64_list_concrete
 QED
 
-Theorem do_eval:
+Theorem recorded_orac_wf_step:
+  recorded_orac_wf compiler orac /\
+  compiler_agrees compiler args (st_v2, bs_v, ws_v) /\
+  (0 < FST (FST (orac 0)) ==> FST (SND args) = (FST (SND (orac 0))))
+  ==>
+  recorded_orac_wf compiler
+    (λj. if j = 0 then ((FST (FST (orac 0)) + 1,0), st_v2, [])
+      else if j = SUC (FST (FST (orac 0))) then args
+      else orac j)
+Proof
+  simp [recorded_orac_wf_def, compiler_agrees_def]
+  \\ simp [GSYM ADD1, seqTheory.LT_SUC]
+  \\ every_case_tac \\ fs []
+  \\ rw [] \\ fs []
+QED
+
+Theorem do_eval_sim:
   do_eval (REVERSE xs) s.eval_state = SOME (env, decs, es) /\
-  s_rel (s : 'a semanticPrimitives$state) t /\
+  s_rel init_eds (s : 'a semanticPrimitives$state) t /\
   LIST_REL (v_rel (orac_s t.eval_state)) xs ys ==>
   ? env' es'.
   es_forward (orac_s t.eval_state) (orac_s es') /\
   do_eval (REVERSE ys) t.eval_state = SOME (env', decs, es') /\
   env_rel (v_rel (orac_s es')) env env' /\
-  s_rel (s with eval_state := es) (t with eval_state := es') /\
-  (! s2 t2. s_rel (s2 : 'a semanticPrimitives$state) t2 /\
+  s_rel init_eds (s with eval_state := es) (t with eval_state := es') /\
+  (! s2 t2. s_rel init_eds (s2 : 'a semanticPrimitives$state) t2 /\
     es_forward (orac_s es') (orac_s t2.eval_state) /\
     es_stack_forward (orac_s es') (orac_s t2.eval_state) ==>
     es_forward (orac_s t2.eval_state)
         (orac_s (reset_env_generation t.eval_state t2.eval_state)) /\
-    s_rel
+    s_rel init_eds
         (s2 with eval_state := reset_env_generation s.eval_state s2.eval_state)
         (t2 with eval_state := reset_env_generation t.eval_state t2.eval_state)
     /\
@@ -862,18 +905,20 @@ Proof
   \\ rveq \\ fs []
   \\ simp [add_env_generation_def, add_decs_generation_def, PULL_EXISTS]
   \\ simp [EL_APPEND_EQN]
-  \\ qexists_tac `init_s`
   \\ conj_asm1_tac
   >- (
     simp [es_forward_def]
     \\ simp [lookup_env_def, FORALL_PROD, lem_listTheory.list_index_def]
     \\ simp [bool_case_eq, option_case_eq, EL_APPEND_EQN]
   )
-  \\ rpt strip_tac \\ rw [] \\ fs []
-  \\ imp_res_tac forward_rules
-  \\ simp [FUN_EQ_THM, EQ_SYM_EQ]
+  \\ rpt strip_tac \\ fs []
+  \\ TRY (imp_res_tac forward_rules \\ rw [FUN_EQ_THM, EQ_SYM_EQ]
+    \\ fs [] \\ NO_TAC)
+  >- (
+    drule_then (drule_then irule) recorded_orac_wf_step
+    \\ rw [] \\ fs []
+  )
   \\ fs [reset_env_generation_def]
-  \\ qexists_tac `init_s'`
   \\ simp []
   \\ conj_asm1_tac
   >- (
@@ -883,17 +928,18 @@ Proof
   \\ simp [EQ_SYM_EQ]
   \\ fs [es_stack_forward_def]
   \\ rfs [EL_APPEND_EQN]
+  \\ imp_res_tac forward_rules
 QED
 
-Theorem declare_env:
+Theorem declare_env_sim:
   declare_env s.eval_state env = SOME (v, es) /\
-  s_rel s t /\
+  s_rel init_eds s t /\
   env_rel (v_rel (orac_s t.eval_state)) env env' ==>
   ?v' es2.
   es_forward (orac_s t.eval_state) (orac_s es2) /\
   declare_env t.eval_state env' = SOME (v', es2) /\
   v_rel (orac_s es2) v v' /\
-  s_rel (s with eval_state := es) (t with eval_state := es2) /\
+  s_rel init_eds (s with eval_state := es) (t with eval_state := es2) /\
   es_stack_forward (orac_s t.eval_state) (orac_s es2)
 Proof
   rw [s_rel_def, declare_env_def]
@@ -910,7 +956,6 @@ Proof
     \\ rw [EL_APPEND_EQN, EL_LUPDATE]
   )
   \\ simp [state_component_equality, PULL_EXISTS]
-  \\ qexists_tac `init_s`
   \\ simp [es_stack_forward_def, EL_LUPDATE]
   \\ imp_res_tac forward_rules \\ fs []
 QED
@@ -935,6 +980,33 @@ Proof
   simp [abort_def] \\ every_case_tac \\ simp []
 QED
 
+Definition Case_def:
+  Case X <=> T
+End
+
+Theorem elim_Case:
+  (Case X /\ Y) = Y /\
+  (Case X ==> Y) = Y
+Proof
+  simp [Case_def]
+QED
+
+val case_const = ``Case``
+fun is_app_case t = is_comb t andalso same_const case_const (rator t)
+
+fun setup (q : term quotation, t : tactic) = let
+    val the_concl = Parse.typedTerm q bool
+    val t2 = (t \\ rpt (pop_assum mp_tac))
+    val (goals, validation) = t2 ([], the_concl)
+    fun get_goal q = first (can (rename [q])) goals |> snd
+    fun init thms st = if null (fst st) andalso aconv (snd st) the_concl
+      then ((K (goals, validation)) \\ TRY (MAP_FIRST ACCEPT_TAC thms)) st
+      else failwith "setup tactic: mismatching starting state"
+    val cases = map (find_terms is_app_case o snd) goals
+  in {get_goal = get_goal, concl = fn () => the_concl,
+    cases = cases, init = (init : thm list -> tactic),
+    all_goals = fn () => map snd goals} end
+
 (* case splits for evaluate proofs *)
 val eval_cases_tac =
   fs [pair_case_eq, result_case_eq, error_result_case_eq, bool_case_eq,
@@ -950,7 +1022,7 @@ val forward_tac = MAP_FIRST (drule_then irule)
 
 (* quantifier instantiation based on s_rel, v_rel etc *)
 val insts_tac = rpt (FIRST ([
-      do_xig_inst `s_rel X_s _`,
+      do_xig_inst `s_rel Ig_init_s X_s _`,
       do_xig_inst `env_rel (v_rel Ig_es) X_env _`,
       do_xig_inst `LIST_REL (v_rel Ig_es) X_env _`,
       do_xig_inst `v_rel Ig_es X_v _`,
@@ -964,17 +1036,16 @@ val insts_tac = rpt (FIRST ([
       match_mp_tac abort_imp_intro \\ rw [] \\ fs []
     ]))
 
-
-Theorem compile_correct:
-
+val eval_simulation_setup = setup (`
   (! ^s env exps s' res es t env'.
   evaluate s env exps = (s', res) /\
-  s_rel s t /\
+  s_rel init_eds s t /\
   env_rel (v_rel (orac_s t.eval_state)) env env' /\
+  Case exps /\
   res <> Rerr (Rabort Rtype_error) ==>
   ? es' t' res'.
   evaluate t env' exps = (t', res') /\
-  s_rel s' t' /\
+  s_rel init_eds s' t' /\
   es' = orac_s t'.eval_state /\
   result_rel (LIST_REL (v_rel es')) (v_rel es') res res' /\
   es_forward (orac_s t.eval_state) es' /\
@@ -982,15 +1053,16 @@ Theorem compile_correct:
   /\
   (! ^s env x pes err_x s' res es t env' y err_y.
   evaluate_match s env x pes err_x = (s', res) /\
-  s_rel s t /\
+  s_rel init_eds s t /\
   es = orac_s t.eval_state /\
   env_rel (v_rel es) env env' /\
   v_rel es x y /\
   v_rel es err_x err_y /\
+  Case pes /\
   res <> Rerr (Rabort Rtype_error) ==>
   ?es' t' res'.
   evaluate_match t env' y pes err_y = (t', res') /\
-  s_rel s' t' /\
+  s_rel init_eds s' t' /\
   es' = orac_s t'.eval_state /\
   result_rel (LIST_REL (v_rel es')) (v_rel es') res res' /\
   es_forward es es' /\
@@ -998,304 +1070,271 @@ Theorem compile_correct:
   /\
   (! ^s env decs s' res t env'.
   evaluate_decs s env decs = (s', res) /\
-  s_rel s t /\
+  s_rel init_eds s t /\
   env_rel (v_rel (orac_s t.eval_state)) env env' /\
+  Case (Dlet, decs) /\
   res <> Rerr (Rabort Rtype_error) ==>
   ?es' t' res'.
   evaluate_decs t env' decs = (t', res') /\
-  s_rel s' t' /\
+  s_rel init_eds s' t' /\
   es' = orac_s t'.eval_state /\
   result_rel (env_rel (v_rel es')) (v_rel es') res res' /\
   es_forward (orac_s t.eval_state) es' /\
   (~ abort res' ==> es_stack_forward (orac_s t.eval_state) es'))
-
-Proof
-
+  `,
   ho_match_mp_tac terminationTheory.full_evaluate_ind
   \\ rpt conj_tac
   \\ rpt (gen_tac ORELSE disch_tac)
   \\ fs [terminationTheory.full_evaluate_def]
+  \\ fs [elim_Case]
   \\ rveq \\ fs []
-  >- (
-    insts_tac
-  )
-  >- (
-    eval_cases_tac
-    \\ insts_tac
-  )
-  >- (
-    insts_tac
-  )
-  >- (
-    eval_cases_tac
-    \\ insts_tac
-  )
-  >- (
-    eval_cases_tac
-    \\ insts_tac
-    \\ drule_then assume_tac can_pmatch_all
-    \\ insts_tac
-  )
-  >- (
-    eval_cases_tac
-    \\ insts_tac
-    \\ fs [do_con_check_def, build_conv_def]
-    \\ every_case_tac \\ fs [] \\ rveq \\ fs []
-    \\ rfs [env_rel_def]
-  )
-  >- (
-    eval_cases_tac
-    \\ drule_then drule env_rel_nsLookup_v
-    \\ rw []
-    \\ simp []
-    \\ insts_tac
-  )
-  >- (
-    insts_tac
-  )
+  );
 
+Triviality eval_simulation_App:
+  ^(#get_goal eval_simulation_setup `Case ([App _ _])`)
+Proof
+  rw []
+  \\ reverse (fs [pair_case_eq, result_case_eq] \\ rveq \\ fs [])
+  \\ insts_tac
+  \\ Cases_on `op = Opapp`
   >- (
-    (* App *)
-    reverse (fs [pair_case_eq, result_case_eq] \\ rveq \\ fs [])
-    \\ insts_tac
-    \\ Cases_on `op = Opapp`
-    >- (
-      rveq \\ fs []
-      \\ imp_res_tac s_rel_clock
-      \\ fs [do_opapp_def]
-      \\ eval_cases_tac
-      \\ fs [listTheory.SWAP_REVERSE_SYM, CaseEq "v"] \\ rveq \\ fs []
-      \\ fs [listTheory.SWAP_REVERSE, miscTheory.FST_triple]
-      \\ eval_cases_tac
-      \\ insts_tac
-      \\ rfs [EVAL ``(dec_clock s).eval_state``]
-      \\ first_x_assum (qsubterm_then `evaluate _ _ _` mp_tac)
-      \\ impl_tac \\ rw [] \\ insts_tac
-      \\ irule env_rel_add_nsBind
-      \\ insts_tac
-      \\ simp [build_rec_env_merge, nsAppend_to_nsBindList]
-      \\ irule env_rel_add_nsBindList
-      \\ simp [LIST_REL_MAP1, SIMP_RULE (bool_ss ++ ETA_ss) [] LIST_REL_MAP2]
-      \\ simp [ELIM_UNCURRY, quotient_pairTheory.PAIR_REL_THM, EVERY2_refl]
-    )
-    \\ Cases_on `op = Eval`
-    >- (
-      fs [do_eval_res_def, terminationTheory.evaluate_def, do_con_check_def]
-      \\ fs [option_case_eq, pair_case_eq] \\ rveq \\ fs []
-      \\ drule_then (drule_then drule) do_eval
-      \\ rw []
-      \\ fs []
-      \\ drule_then assume_tac s_rel_clock
-      \\ fs [bool_case_eq] \\ rveq \\ fs []
-      \\ insts_tac
-      \\ fs [EVAL ``(dec_clock x).eval_state``]
-      \\ eval_cases_tac
-      \\ insts_tac
-      \\ TRY (drule_then (qsubterm_then `declare_env _ _` mp_tac) declare_env
-        \\ impl_tac \\ rw []
-        \\ TRY (irule env_rel_extend_dec_env))
-      \\ insts_tac
-      \\ first_x_assum drule \\ impl_tac
-      \\ rw [] \\ insts_tac
-    )
+    rveq \\ fs []
+    \\ imp_res_tac s_rel_clock
+    \\ fs [do_opapp_def]
     \\ eval_cases_tac
-    \\ drule_then assume_tac do_app
-    \\ insts_tac
-    \\ fs [s_rel_def] \\ rveq \\ fs []
-    \\ simp [state_component_equality]
-    \\ qexists_tac `init_s'`
-    \\ simp []
-  )
-
-  >- (
-    eval_cases_tac
-    \\ insts_tac
-    \\ fs [do_log_def]
-    \\ eval_cases_tac
-    \\ rveq \\ fs []
-    \\ insts_tac
-  )
-
-  >- (
-    eval_cases_tac
-    \\ insts_tac
-    \\ fs [do_if_def]
+    \\ fs [listTheory.SWAP_REVERSE_SYM, CaseEq "v"] \\ rveq \\ fs []
+    \\ fs [listTheory.SWAP_REVERSE, miscTheory.FST_triple]
     \\ eval_cases_tac
     \\ insts_tac
-   )
-
-  >- (
-    eval_cases_tac
-    \\ insts_tac
-    \\ drule_then assume_tac can_pmatch_all
-    \\ insts_tac
-    \\ fs [bind_exn_v_def]
-    \\ insts_tac
-  )
-
-  >- (
-    eval_cases_tac
-    \\ insts_tac
+    \\ rfs [EVAL ``(dec_clock s).eval_state``]
     \\ first_x_assum (qsubterm_then `evaluate _ _ _` mp_tac)
     \\ impl_tac \\ rw [] \\ insts_tac
-    \\ simp [namespaceTheory.nsOptBind_def]
-    \\ CASE_TAC \\ fs []
-    \\ insts_tac
     \\ irule env_rel_add_nsBind
     \\ insts_tac
-  )
-
-  >- (
-    eval_cases_tac
-    \\ insts_tac
-    \\ fs [miscTheory.FST_triple, MAP_MAP_o]
-    \\ fs [GSYM pairarg_to_pair_map, ELIM_UNCURRY, o_DEF, ETA_THM]
-    \\ first_x_assum (qsubterm_then `evaluate _ _ _` mp_tac)
-    \\ impl_tac \\ rw [] \\ insts_tac
     \\ simp [build_rec_env_merge, nsAppend_to_nsBindList]
     \\ irule env_rel_add_nsBindList
     \\ simp [LIST_REL_MAP1, SIMP_RULE (bool_ss ++ ETA_ss) [] LIST_REL_MAP2]
-    \\ simp [quotient_pairTheory.PAIR_REL_THM, ELIM_UNCURRY]
-    \\ simp [GSYM pairarg_to_pair_map, ELIM_UNCURRY, EVERY2_refl]
+    \\ simp [ELIM_UNCURRY, quotient_pairTheory.PAIR_REL_THM, EVERY2_refl]
   )
-
+  \\ Cases_on `op = Eval`
   >- (
-    insts_tac
-  )
-
-  >- (
-    fs [bool_case_eq]
-    \\ insts_tac
-    \\ drule_then (qsubterm_then `pmatch _ _ _ _ _` mp_tac) pmatch_use
-    \\ rpt (disch_then drule)
-    \\ eval_cases_tac
-    \\ fs [match_result_rel_def]
+    fs [do_eval_res_def, terminationTheory.evaluate_def, do_con_check_def]
+    \\ fs [option_case_eq, pair_case_eq] \\ rveq \\ fs []
+    \\ drule_then (drule_then drule) do_eval_sim
     \\ rw []
+    \\ fs []
+    \\ drule_then assume_tac s_rel_clock
+    \\ fs [bool_case_eq] \\ rveq \\ fs []
     \\ insts_tac
-    \\ first_x_assum (qsubterm_then `evaluate _ _ _` mp_tac)
-    \\ impl_tac \\ rw [] \\ insts_tac
-    \\ simp [nsAppend_to_nsBindList]
-    \\ irule env_rel_add_nsBindList
-    \\ simp [nsAppend_to_nsBindList]
-  )
-
-  >- (
-    insts_tac
-  )
-
-  >- (
-    eval_cases_tac
+    \\ fs [EVAL ``(dec_clock x).eval_state``]
+    \\ eval_cases_tac
     \\ insts_tac
-    \\ first_x_assum (qsubterm_then `evaluate_decs _ _ _` mp_tac)
-    \\ impl_tac \\ rw [] \\ insts_tac
-    \\ TRY (irule env_rel_extend_dec_env)
+    \\ TRY (drule_then (drule_then (qsubterm_then `declare_env _ _` mp_tac))
+        declare_env_sim
+      \\ impl_tac
+      \\ (irule env_rel_extend_dec_env ORELSE disch_tac))
     \\ insts_tac
-    \\ TRY strip_tac
-    \\ fs [combine_dec_result_def]
-    \\ every_case_tac \\ fs []
+    \\ first_x_assum drule \\ impl_tac
     \\ rw [] \\ insts_tac
-    \\ simp [GSYM (SIMP_RULE (srw_ss ()) [] extend_dec_env_def)]
-    \\ TRY (irule env_rel_extend_dec_env)
+  )
+  \\ eval_cases_tac
+  \\ drule_then (drule_then assume_tac) do_app_sim
+  \\ insts_tac
+  \\ fs [s_rel_def] \\ rveq \\ fs []
+  \\ simp [state_component_equality]
+QED
+
+Triviality eval_simulation_Denv:
+  ^(#get_goal eval_simulation_setup `Case (_, [Denv _])`)
+Proof
+  rw []
+  \\ eval_cases_tac
+  \\ fs [declare_env_def, s_rel_def]
+  \\ rveq \\ fs []
+  \\ fs [pair_case_eq]
+  \\ rveq \\ fs []
+  \\ simp [lem_listTheory.list_index_def]
+  \\ simp [state_component_equality]
+  \\ qmatch_goalsub_abbrev_tac `es_forward cur_es new_es`
+  \\ qsuff_tac `es_forward cur_es new_es`
+  >- (
+    rpt strip_tac \\ insts_tac
+    \\ simp [EL_LUPDATE]
+    \\ insts_tac
+    \\ simp [nsSing_eq_bind]
+    \\ fs [markerTheory.Abbrev_def, es_stack_forward_def, EL_LUPDATE]
+    \\ irule env_rel_add_nsBind
+    \\ simp [v_to_env_id_def, v_to_nat_def, nat_to_v_def]
+    \\ fs [markerTheory.Abbrev_def, lookup_env_def,
+          lem_listTheory.list_index_def, EL_LUPDATE, EL_APPEND_EQN,
+          es_stack_forward_def]
     \\ insts_tac
   )
-
   >- (
-    fs [bool_case_eq, pair_case_eq, result_case_eq]
+    fs [markerTheory.Abbrev_def, es_forward_def, FORALL_PROD]
+    \\ simp [lookup_env_def, lem_listTheory.list_index_def, option_case_eq]
+    \\ simp [EL_LUPDATE]
+    \\ rw [EL_APPEND_EQN]
+  )
+QED
+
+Triviality eval_simulation_Con:
+  ^(#get_goal eval_simulation_setup `Case ([Con _ _])`)
+Proof
+  rpt disch_tac
+  \\ eval_cases_tac
+  \\ insts_tac
+  \\ imp_res_tac env_rel_def
+  \\ fs [do_con_check_def, build_conv_def]
+  \\ every_case_tac
+  \\ insts_tac
+QED
+
+Triviality eval_simulation_Let:
+  ^(#get_goal eval_simulation_setup `Case ([Let _ _ _])`)
+Proof
+  rpt disch_tac
+  \\ eval_cases_tac
+  \\ insts_tac
+  \\ first_x_assum (qsubterm_then `evaluate _ _ _` mp_tac)
+  \\ simp [namespaceTheory.nsOptBind_def]
+  \\ CASE_TAC \\ fs []
+  \\ impl_tac
+  \\ rw []
+  \\ insts_tac
+  \\ irule env_rel_add_nsBind
+  \\ insts_tac
+QED
+
+Triviality eval_simulation_Letrec:
+  ^(#get_goal eval_simulation_setup `Case ([Letrec _ _])`)
+Proof
+  rpt disch_tac
+  \\ eval_cases_tac
+  \\ insts_tac
+  \\ fs [miscTheory.FST_triple, MAP_MAP_o]
+  \\ fs [GSYM pairarg_to_pair_map, ELIM_UNCURRY, o_DEF, ETA_THM]
+  \\ first_x_assum (qsubterm_then `evaluate _ _ _` mp_tac)
+  \\ impl_tac \\ rw [] \\ insts_tac
+  \\ simp [build_rec_env_merge, nsAppend_to_nsBindList]
+  \\ irule env_rel_add_nsBindList
+  \\ simp [LIST_REL_MAP1, SIMP_RULE (bool_ss ++ ETA_ss) [] LIST_REL_MAP2]
+  \\ simp [quotient_pairTheory.PAIR_REL_THM, ELIM_UNCURRY]
+  \\ simp [GSYM pairarg_to_pair_map, ELIM_UNCURRY, EVERY2_refl]
+QED
+
+Triviality eval_simulation_match:
+  ^(#get_goal eval_simulation_setup `Case ((_, _) :: _)`)
+Proof
+  rpt disch_tac
+  \\ eval_cases_tac
+  \\ drule_then (drule_then assume_tac) pmatch_drule_form
+  \\ insts_tac
+  \\ fs [match_result_rel_def]
+  \\ insts_tac
+  \\ first_x_assum (qsubterm_then `evaluate _ _ _` mp_tac)
+  \\ impl_tac \\ rw [] \\ insts_tac
+  \\ simp [nsAppend_to_nsBindList]
+  \\ irule env_rel_add_nsBindList
+  \\ simp [nsAppend_to_nsBindList]
+QED
+
+Triviality eval_simulation_cons_decs:
+  ^(#get_goal eval_simulation_setup `Case (Dlet, _ :: _ :: _)`)
+Proof
+  rpt disch_tac
+  \\ eval_cases_tac
+  \\ insts_tac
+  \\ first_x_assum (qsubterm_then `evaluate_decs _ _ _` mp_tac)
+  \\ impl_tac \\ rw [] \\ insts_tac
+  \\ TRY (irule env_rel_extend_dec_env)
+  \\ insts_tac
+  \\ TRY strip_tac
+  \\ fs [combine_dec_result_def]
+  \\ every_case_tac \\ fs []
+  \\ rw [] \\ insts_tac
+  \\ simp [GSYM (SIMP_RULE (srw_ss ()) [] extend_dec_env_def)]
+  \\ TRY (irule env_rel_extend_dec_env)
+  \\ insts_tac
+QED
+
+Triviality eval_simulation_Dletrec:
+  ^(#get_goal eval_simulation_setup `Case (_, [Dletrec _ _])`)
+Proof
+  rpt disch_tac
+  \\ eval_cases_tac
+  \\ insts_tac
+  \\ fs [miscTheory.FST_triple, MAP_MAP_o, o_DEF, ELIM_UNCURRY, ETA_THM]
+  \\ simp [build_rec_env_merge, nsAppend_to_nsBindList]
+  \\ irule env_rel_add_nsBindList
+  \\ simp []
+  \\ simp [LIST_REL_MAP1, SIMP_RULE (bool_ss ++ ETA_ss) [] LIST_REL_MAP2]
+  \\ simp [quotient_pairTheory.PAIR_REL_THM, ELIM_UNCURRY]
+  \\ simp [EVERY2_refl]
+QED
+
+Triviality eval_simulation_Dtype:
+  ^(#get_goal eval_simulation_setup `Case (_, [Dtype _ _])`)
+Proof
+  rpt disch_tac
+  \\ eval_cases_tac
+  \\ fs [EVERY_MEM, FORALL_PROD, MEM_MAP, EXISTS_PROD, PULL_EXISTS,
+      terminationTheory.check_dup_ctors_thm]
+  \\ fs [s_rel_def, state_component_equality]
+  \\ insts_tac
+  \\ simp []
+QED
+
+Triviality eval_simulation_Dexn:
+  ^(#get_goal eval_simulation_setup `Case (_, [Dexn _ _ _])`)
+Proof
+  rpt disch_tac
+  \\ eval_cases_tac
+  \\ fs [s_rel_def, state_component_equality]
+  \\ insts_tac
+QED
+
+Triviality eval_simulation_Dlocal:
+  ^(#get_goal eval_simulation_setup `Case (_, [Dlocal _ _])`)
+Proof
+  rpt disch_tac
+  \\ eval_cases_tac
+  \\ insts_tac
+  \\ first_x_assum (qsubterm_then `evaluate_decs _ _ _` mp_tac)
+  \\ impl_tac \\ rw [] \\ insts_tac
+  \\ irule env_rel_extend_dec_env
+  \\ insts_tac
+QED
+
+Theorem eval_simulation:
+  ^(#concl eval_simulation_setup ())
+Proof
+  #init eval_simulation_setup [eval_simulation_App,
+    eval_simulation_Denv, eval_simulation_Con, eval_simulation_Let,
+    eval_simulation_Letrec, eval_simulation_match,
+    eval_simulation_cons_decs, eval_simulation_Dletrec,
+    eval_simulation_Dtype, eval_simulation_Dexn, eval_simulation_Dlocal]
+  \\ rpt disch_tac
+  \\ insts_tac
+  \\ TRY ( (
+    (* big hammer for similar cases *)
+    eval_cases_tac
+    \\ fs [elim_Case]
     \\ insts_tac
-    \\ imp_res_tac evaluate_sing
-    \\ rveq \\ fs []
-    \\ drule_then (qsubterm_then `pmatch _ _ _ _ _` mp_tac) pmatch_use
-    (* FIXME: why doesn't this work?
-    \\ disch_then (qsubterm_then `pmatch _ s'.refs _ _ _` mp_tac)
-    *)
-    \\ imp_res_tac (List.nth (CONJUNCTS forward_rules, 2))
-    \\ rpt (disch_then drule)
-    \\ every_case_tac \\ fs [match_result_rel_def, bind_exn_v_def]
-    \\ rw [alist_to_ns_to_bind2]
-    \\ irule env_rel_add_nsBindList
+    \\ fs [do_con_check_def, build_conv_def, do_log_def, do_if_def]
+    \\ TRY (drule_then (drule_then assume_tac) can_pmatch_all)
+    \\ TRY (drule_then (drule_then assume_tac)
+        (REWRITE_RULE [match_result_rel_def] pmatch_drule_form))
+    \\ TRY (drule_then drule env_rel_nsLookup_v \\ rw [])
+    \\ eval_cases_tac
+    \\ fs [bind_exn_v_def]
+    \\ insts_tac
+    \\ simp [alist_to_ns_to_bind2]
+    \\ TRY (irule env_rel_add_nsBindList)
+    \\ TRY (irule env_rel_nsLift)
     \\ simp []
-  )
-
-  >- (
-    eval_cases_tac
-    \\ insts_tac
-    \\ fs [miscTheory.FST_triple, MAP_MAP_o, o_DEF, ELIM_UNCURRY, ETA_THM]
-    \\ simp [build_rec_env_merge, nsAppend_to_nsBindList]
-    \\ irule env_rel_add_nsBindList
-    \\ simp []
-    \\ simp [LIST_REL_MAP1, SIMP_RULE (bool_ss ++ ETA_ss) [] LIST_REL_MAP2]
-    \\ simp [quotient_pairTheory.PAIR_REL_THM, ELIM_UNCURRY]
-    \\ simp [EVERY2_refl]
-  )
-
-  >- (
-    eval_cases_tac
-    \\ fs [EVERY_MEM, FORALL_PROD, MEM_MAP, EXISTS_PROD, PULL_EXISTS,
-        terminationTheory.check_dup_ctors_thm]
-    \\ fs [s_rel_def, state_component_equality]
-    \\ insts_tac
-    \\ qexists_tac `init_s`
-    \\ simp []
-  )
-
-  >- (
-    insts_tac
-  )
-
-  >- (
-    (* Denv *)
-    eval_cases_tac
-    \\ fs [declare_env_def, s_rel_def]
-    \\ rveq \\ fs []
-    \\ fs [pair_case_eq]
-    \\ rveq \\ fs []
-    \\ simp [lem_listTheory.list_index_def]
-    \\ simp [state_component_equality]
-    \\ qmatch_goalsub_abbrev_tac `es_forward cur_es new_es`
-    \\ qsuff_tac `es_forward cur_es new_es`
-    >- (
-      rpt strip_tac \\ insts_tac
-      \\ TRY (qexists_tac `init_s` \\ simp [])
-      \\ simp [EL_LUPDATE]
-      \\ insts_tac
-      \\ simp [nsSing_eq_bind]
-      \\ fs [markerTheory.Abbrev_def, es_stack_forward_def, EL_LUPDATE]
-      \\ irule env_rel_add_nsBind
-      \\ simp [v_to_env_id_def, v_to_nat_def, nat_to_v_def]
-      \\ fs [markerTheory.Abbrev_def, lookup_env_def,
-            lem_listTheory.list_index_def, EL_LUPDATE, EL_APPEND_EQN,
-            es_stack_forward_def]
-      \\ insts_tac
-    )
-    >- (
-      fs [markerTheory.Abbrev_def, es_forward_def, FORALL_PROD]
-      \\ simp [lookup_env_def, lem_listTheory.list_index_def, option_case_eq]
-      \\ simp [EL_LUPDATE]
-      \\ rw [EL_APPEND_EQN]
-    )
-  )
-
-  >- (
-    insts_tac
-    \\ fs [s_rel_def, state_component_equality]
-    \\ qexists_tac `init_s` \\ simp []
-  )
-
-  >- (
-    eval_cases_tac
-    \\ insts_tac
-    \\ irule env_rel_nsLift
-    \\ fs [env_rel_def]
-    \\ rw [] \\ res_tac
-  )
-
-  >- (
-    eval_cases_tac
-    \\ insts_tac
-    \\ first_x_assum (qsubterm_then `evaluate_decs _ _ _` mp_tac)
-    \\ impl_tac \\ rw [] \\ insts_tac
-    \\ irule env_rel_extend_dec_env
-    \\ insts_tac
+   )
+  \\ NO_TAC
   )
 QED
 
@@ -1333,9 +1372,10 @@ End
 Definition record_forward_def:
   record_forward es es' = (case es of
     | SOME (EvalOracle s) => ?s'. es' = SOME (EvalOracle s') /\
-          (FST (FST (s.oracle 0)) <= FST (FST (s'.oracle 0))) /\
-          (!j. 0 < j /\ j < FST (FST (s.oracle 0)) + 1 ==> s'.oracle j = s.oracle j)
-    | _ => ~ (?s'. es' = SOME (EvalOracle s'))
+        (FST (FST (s.oracle 0)) <= FST (FST (s'.oracle 0))) /\
+        (!j. 0 < j /\ j < FST (FST (s.oracle 0)) + 1 ==>
+            s'.oracle j = s.oracle j)
+    | _ => (case es' of SOME (EvalOracle _) => F | _ => T)
   )
 End
 
@@ -1361,22 +1401,22 @@ Proof
 QED
 
 Definition is_record_def:
-  is_record f es ⇔ case es of
+  is_record f init_s es ⇔ case es of
     | SOME (EvalOracle s) =>
-        ∃init_s. s.custom_do_eval = do_eval_record f init_s
+        s.custom_do_eval = do_eval_record f init_s
     | _ => F
 End
 
 Theorem is_record_IMP:
-  is_record f es ==> ? orac_st. es = SOME (EvalOracle orac_st)
+  is_record f init_s es ==> ? orac_st. es = SOME (EvalOracle orac_st)
 Proof
   simp [is_record_def] \\ every_case_tac \\ simp []
 QED
 
 Theorem insert_do_eval:
   do_eval vs es = SOME (env, decs, es') /\
-  is_record f es ==>
-  is_record f es' /\
+  is_record f init_s es ==>
+  is_record f init_s es' /\
   record_forward es es' /\
   (orac_agrees orac es' ==>
   do_eval vs (insert_oracle f orac es) = SOME (env, decs,
@@ -1386,7 +1426,6 @@ Proof
   \\ disch_tac
   \\ fs [option_case_eq, eval_state_case_eq, pair_case_eq] \\ rveq \\ fs []
   \\ fs [PULL_EXISTS]
-  \\ qexists_tac `init_s`
   \\ fs [do_eval_def, add_env_generation_def, insert_oracle_def]
   \\ fs [do_eval_record_def, list_case_eq, option_case_eq] \\ rveq \\ fs []
   \\ rpt (pairarg_tac \\ fs [])
@@ -1401,8 +1440,8 @@ QED
 
 Theorem insert_declare_env:
   declare_env es1 env = SOME (x, es2) /\
-  is_record f es1 ==>
-  is_record f es2 /\
+  is_record f init_s es1 ==>
+  is_record f init_s es2 /\
   record_forward es1 es2 /\
   (orac_agrees orac es2 ==>
   declare_env (insert_oracle f orac es1) env = SOME (x,
@@ -1413,12 +1452,11 @@ Proof
   \\ disch_tac
   \\ fs [] \\ rveq \\ fs []
   \\ simp [PULL_EXISTS]
-  \\ qexists_tac `init_s`
   \\ simp [record_forward_def]
 QED
 
 Theorem reset_env_generation_orac_eqs:
-  (is_record f (reset_env_generation es2 es3) = is_record f es3) ∧
+  (is_record f x (reset_env_generation es2 es3) = is_record f x es3) ∧
   (record_forward es1 (reset_env_generation es2 es3) = record_forward es1 es3) ∧
   (orac_agrees orac (reset_env_generation es2 es3) = orac_agrees orac es3) ∧
   (reset_env_generation (insert_oracle f orac es1) es2 =
@@ -1437,29 +1475,29 @@ Triviality record_forward_trans_sym
 Theorem evaluate_is_record_forward:
   (! ^s env exps s' res.
   evaluate s env exps = (s', res) /\
-  is_record f s.eval_state
+  is_record f init_s s.eval_state
   ==>
-  is_record f s'.eval_state /\
+  is_record f init_s s'.eval_state /\
   record_forward s.eval_state s'.eval_state)
   /\
   (! ^s env x pes err_x s' res.
   evaluate_match s env x pes err_x = (s', res) /\
-  is_record f s.eval_state
+  is_record f init_s s.eval_state
   ==>
-  is_record f s'.eval_state /\
+  is_record f init_s s'.eval_state /\
   record_forward s.eval_state s'.eval_state)
   /\
   (! ^s env decs s' res.
   evaluate_decs s env decs = (s', res) /\
-  is_record f s.eval_state
+  is_record f init_s s.eval_state
   ==>
-  is_record f s'.eval_state /\
+  is_record f init_s s'.eval_state /\
   record_forward s.eval_state s'.eval_state)
 Proof
   ho_match_mp_tac terminationTheory.full_evaluate_ind
   \\ rpt conj_tac
   \\ rpt (gen_tac ORELSE disch_tac)
-  \\ fs [compile_exp_def, compile_dec_def, terminationTheory.full_evaluate_def]
+  \\ fs [terminationTheory.full_evaluate_def]
   \\ rveq \\ fs []
   \\ simp [record_forward_refl]
   \\ fs [pair_case_eq, option_case_eq, result_case_eq] \\ rveq \\ fs []
@@ -1478,33 +1516,6 @@ Proof
   \\ simp [record_forward_refl]
 QED
 
-Definition Case_def:
-  Case X <=> T
-End
-
-Theorem elim_Case:
-  (Case X /\ Y) = Y /\
-  (Case X ==> Y) = Y
-Proof
-  simp [Case_def]
-QED
-
-val case_const = ``Case``
-fun is_app_case t = is_comb t andalso same_const case_const (rator t)
-
-fun setup (q : term quotation, t : tactic) = let
-    val the_concl = Parse.typedTerm q bool
-    val t2 = (t \\ rpt (pop_assum mp_tac))
-    val (goals, validation) = t2 ([], the_concl)
-    fun get_goal q = first (can (rename [q])) goals |> snd
-    fun init thms st = if null (fst st) andalso aconv (snd st) the_concl
-      then ((K (goals, validation)) \\ TRY (MAP_FIRST ACCEPT_TAC thms)) st
-      else failwith "setup tactic: mismatching starting state"
-    val cases = map (find_terms is_app_case o snd) goals
-  in {get_goal = get_goal, concl = fn () => the_concl,
-    cases = cases, init = (init : thm list -> tactic),
-    all_goals = fn () => map snd goals} end
-
 val agrees_tac = (drule_then irule orac_agrees_backward)
   \\ rpt (simp_tac bool_ss [record_forward_refl]
     \\ drule_then irule record_forward_trans_sym)
@@ -1521,7 +1532,7 @@ fun imp_res_simp_tac t = IMP_RES_THEN mp_tac t
 val insert_oracle_correct_setup = setup (
   `(! ^s env exps s' res.
   evaluate s env exps = (s', res) /\
-  is_record f s.eval_state /\
+  is_record f init_s s.eval_state /\
   orac_agrees orac s'.eval_state /\
   Case (Let, exps) /\
   res <> Rerr (Rabort Rtype_error)
@@ -1532,7 +1543,7 @@ val insert_oracle_correct_setup = setup (
   /\
   (! ^s env x pes err_x s' res.
   evaluate_match s env x pes err_x = (s', res) /\
-  is_record f s.eval_state /\
+  is_record f init_s s.eval_state /\
   orac_agrees orac s'.eval_state /\
   Case (Mat, pes) /\
   res <> Rerr (Rabort Rtype_error)
@@ -1544,7 +1555,7 @@ val insert_oracle_correct_setup = setup (
   /\
   (! ^s env decs s' res.
   evaluate_decs s env decs = (s', res) /\
-  is_record f s.eval_state /\
+  is_record f init_s s.eval_state /\
   orac_agrees orac s'.eval_state /\
   Case (Dlet, decs) /\
   res <> Rerr (Rabort Rtype_error)
@@ -1555,7 +1566,7 @@ val insert_oracle_correct_setup = setup (
   ho_match_mp_tac terminationTheory.full_evaluate_ind
   \\ rpt conj_tac
   \\ rpt (gen_tac ORELSE disch_tac)
-  \\ fs [compile_exp_def, compile_dec_def, terminationTheory.full_evaluate_def]
+  \\ fs [terminationTheory.full_evaluate_def]
   \\ fs [elim_Case]
   \\ rveq \\ fs []
   );
@@ -1582,7 +1593,7 @@ Proof
     \\ fs [option_case_eq, pair_case_eq] \\ rveq \\ fs []
     \\ drule insert_do_eval
     \\ rpt (disch_then drule)
-    \\ disch_then (qspecl_then [`orac`, `f`] mp_tac)
+    \\ disch_then (qspecl_then [`orac`, `init_s`, `f`] mp_tac)
     \\ rw []
     \\ imp_res_simp_tac evaluate_is_record_forward
     \\ fs [bool_case_eq] \\ rveq \\ fs []
@@ -1666,7 +1677,7 @@ QED
 Theorem evaluate_record_suffix:
   (! ^s env exps s' res.
   evaluate s env exps = (s', res) /\
-  is_record f s.eval_state /\
+  is_record f init_s s.eval_state /\
   k <= s.clock
   ==>
   let ev = evaluate (s with clock updated_by (\c. c - k)) env exps in
@@ -1680,7 +1691,7 @@ Theorem evaluate_record_suffix:
   /\
   (! ^s env x pes err_x s' res.
   evaluate_match s env x pes err_x = (s', res) /\
-  is_record f s.eval_state /\
+  is_record f init_s s.eval_state /\
   k <= s.clock
   ==>
   let ev = evaluate_match (s with clock updated_by (\c. c - k)) env x pes err_x in
@@ -1694,7 +1705,7 @@ Theorem evaluate_record_suffix:
   /\
   (! ^s env decs s' res.
   evaluate_decs s env decs = (s', res) /\
-  is_record f s.eval_state /\
+  is_record f init_s s.eval_state /\
   k <= s.clock
   ==>
   let ev = evaluate_decs (s with clock updated_by (\c. c - k)) env decs in
@@ -1709,7 +1720,7 @@ Proof
   ho_match_mp_tac terminationTheory.full_evaluate_ind
   \\ rpt conj_tac
   \\ rpt (gen_tac ORELSE disch_tac)
-  \\ fs [compile_exp_def, compile_dec_def, terminationTheory.full_evaluate_def]
+  \\ fs [terminationTheory.full_evaluate_def]
   \\ rveq \\ fs []
   \\ simp [record_forward_refl]
   \\ fs [do_eval_res_def]
@@ -1732,22 +1743,26 @@ Proof
 QED
 
 Definition mk_eval_oracle_def:
-  mk_eval_oracle s env decs = (\n.
+  mk_eval_oracle compiler st0 s env decs n =
     case (OLEAST k. ?s' res.
       evaluate_decs (s with clock := k) env decs = (s', res) /\
         n < FST (FST ((orac_s (s'.eval_state)).oracle 0))
     ) of
-    | NONE => ((0, 0), Conv NONE [], [])
+    | NONE => if n = 0
+        then ((0, 0), st0, [])
+        else let (env_id, s_v, decs) = mk_eval_oracle compiler st0 s
+                env decs (n - 1) in
+            let (s_v2, _, _) = compiler (env_id, s_v, decs) in
+            ((0, 0), s_v2, [])
     | SOME k =>
       let (s', _) = evaluate_decs (s with clock := k) env decs in
         (orac_s s'.eval_state).oracle (n + 1)
-  )
 End
 
 Theorem evaluate_decs_clock_record_common_prefix:
   evaluate_decs s env decs = (s', res) /\
   evaluate_decs (s with clock := k) env decs = (s'', res') /\
-  is_record f s.eval_state /\
+  is_record f init_s s.eval_state /\
   j < FST (FST ((orac_s s'.eval_state).oracle 0)) /\
   j < FST (FST ((orac_s s''.eval_state).oracle 0)) ==>
   (orac_s s'.eval_state).oracle (j + 1) =
@@ -1787,39 +1802,60 @@ QED
 
 Theorem mk_eval_oracle_agrees:
   evaluate_decs (t with clock := k) env decs = (t', res) /\
-  s_rel s t ==>
-  orac_agrees (mk_eval_oracle t env decs) (t'.eval_state)
+  s_rel init_eds s t ==>
+  orac_agrees (mk_eval_oracle compiler st0 t env decs) (t'.eval_state)
 Proof
   rw [s_rel_def, orac_agrees_def]
-  \\ `is_record dec_s.compiler (SOME (EvalOracle orac_s'))`
-    by (simp [is_record_def] \\ metis_tac [])
+  \\ `is_record init_eds.compiler init_eds.compiler_state
+        (SOME (EvalOracle orac_s'))`
+    by (simp [is_record_def] )
   \\ imp_res_simp_tac evaluate_is_record_forward
   \\ imp_res_simp_tac is_record_IMP
   \\ fs []
   \\ rw []
-  \\ simp [mk_eval_oracle_def]
+  \\ simp [Once mk_eval_oracle_def]
   \\ DEEP_INTRO_TAC whileTheory.OLEAST_INTRO
   \\ rw []
   >- (
     first_x_assum (qspec_then `k` mp_tac)
     \\ simp []
   )
-  \\ fs []
-  \\ dxrule evaluate_decs_clock_record_common_prefix
-  \\ simp []
-  \\ rpt (disch_then drule)
-  \\ simp []
+  >- (
+    first_x_assum (qspec_then `k` mp_tac)
+    \\ simp []
+  )
+  >- (
+    fs []
+    \\ dxrule evaluate_decs_clock_record_common_prefix
+    \\ simp []
+    \\ rpt (disch_then drule)
+    \\ simp []
+  )
 QED
 
+Definition mk_dummy_orac_def:
+  mk_dummy_orac compiler st0 (0 : num) =
+    (((0, 0), st0, []) : compiler_args) /\
+  mk_dummy_orac compiler st0 (SUC j) =
+    ((0, 0), FST (compiler (mk_dummy_orac compiler st0 j)), [])
+End
+
 Definition mk_orac_st_def:
-  mk_orac_st eds s env decs =
+  mk_orac_st compiler st0 s env decs = (case s.eval_state of
+    | NONE => SOME (EvalOracle <|
+      oracle := mk_dummy_orac compiler st0 ;
+      custom_do_eval := K (K NONE) ;
+      envs := [[]]; generation := 0 |>)
+    | SOME (EvalOracle _) => NONE
+    | SOME (EvalDecs eds) =>
     let es_record = EvalOracle <|
       oracle := K ((0,0),Conv NONE [],[]);
       custom_do_eval := do_eval_record eds.compiler eds.compiler_state;
       envs := [[]]; generation := 0|> in
-    let orac = mk_eval_oracle (s with eval_state := SOME es_record)
-      env decs in
+    let orac = mk_eval_oracle compiler st0
+        (s with eval_state := SOME es_record) env decs in
     insert_oracle eds.compiler orac (SOME es_record)
+  )
 End
 
 Theorem result_rel_IMP_cases:
@@ -1830,43 +1866,73 @@ Proof
   \\ Cases_on `e` \\ simp []
 QED
 
+Theorem s_rel_clock2:
+  !k. s_rel init_eds s t ==> s_rel init_eds (s with clock := k) (t with clock := k)
+Proof
+  rw [s_rel_def]
+  \\ simp [semanticPrimitivesTheory.state_component_equality]
+  \\ simp []
+QED
+
+Definition init_eval_state_def:
+  init_eval_state es = (case es of
+    | NONE => T
+    | SOME (EvalDecs eds) => eds.env_id_counter = (0, 0, 1)
+    | SOME (EvalOracle _) => F
+  )
+End
+
+Theorem evaluate_no_eval_simulation:
+  evaluate_decs s env decs = (s', r) /\
+  r <> Rerr (Rabort Rtype_error) /\
+  s.eval_state = NONE ==>
+  evaluate_decs (s with eval_state := es) env decs = (s', r)
+
+Proof
+  cheat
+QED
+
 Theorem evaluate_prog_with_clock_mk_orac_st:
   evaluate_prog_with_clock s1 env k decs = (ffi, res) /\
   res <> Rerr (Rabort Rtype_error) /\
-  s1.eval_state = SOME (EvalDecs eds) /\
+  init_eval_state s1.eval_state /\
   s1.refs = [] /\
-  nsAll (K concrete_v) env.v /\
-  eds.env_id_counter = (0, 0, 1) ==>
+  nsAll (K concrete_v) env.v ==>
   ?res'.
-  evaluate_prog_with_clock (s1 with eval_state := mk_orac_st eds s1 env decs)
+  evaluate_prog_with_clock
+    (s1 with eval_state := mk_orac_st c st0 s1 env decs)
     env k decs = (ffi, res') /\
   result_rel (K (K T)) (K (K T)) res res'
 Proof
-  simp [evaluate_prog_with_clock_def]
-  \\ simp_tac bool_ss [mk_orac_st_def]
-  \\ rpt (pairarg_tac \\ full_simp_tac bool_ss [UNCURRY_DEF])
-  \\ pop_assum mp_tac
-  \\ LET_ELIM_TAC
+  simp [evaluate_prog_with_clock_def, mk_orac_st_def, init_eval_state_def]
+  \\ every_case_tac
+  \\ rpt disch_tac
+  \\ rpt (pairarg_tac \\ fs [])
+  >- (
+    imp_res_tac evaluate_no_eval_simulation
+    \\ rfs []
+    \\ rveq \\ fs []
+  )
   \\ rveq \\ fs []
-  \\ rveq \\ fs []
-  \\ `s_rel (s1 with clock := k)
-    (s1 with <| clock := k; eval_state := SOME es_record |>)`
-  by ( unabbrev_all_tac \\ simp [s_rel_def, state_component_equality] )
-  \\ drule_then drule (List.last (CONJUNCTS compile_correct))
-  \\ simp []
+  \\ qmatch_asmsub_abbrev_tac `SOME (EvalOracle orac_st)`
+  \\ `s_rel e s1 (s1 with <| eval_state := SOME (EvalOracle orac_st) |>)`
+  by ( unabbrev_all_tac
+    \\ simp [s_rel_def, state_component_equality, recorded_orac_wf_def] )
+  \\ drule_then (qspec_then `k` assume_tac) s_rel_clock2
+  \\ drule_then drule (List.last (CONJUNCTS eval_simulation))
+  \\ simp [Case_def]
   \\ disch_then (qspec_then `env` mp_tac)
   \\ simp [env_rel_concrete_v]
   \\ disch_tac \\ fs []
   \\ drule (List.last (CONJUNCTS insert_oracle_correct))
-  \\ disch_then (qspecl_then [`orac`, `eds.compiler`] mp_tac)
-  \\ `s_rel s1 (s1 with <| eval_state := SOME es_record |>)`
-  by ( unabbrev_all_tac \\ simp [s_rel_def, state_component_equality] )
-  \\ fs [Case_def, markerTheory.Abbrev_def]
-  \\ rveq \\ fs []
+  \\ simp []
+  \\ disch_then (qsubterm_then `evaluate_decs _ _` mp_tac)
+  \\ simp [GSYM PULL_EXISTS, is_record_def]
   \\ impl_tac >- (
-    drule_then drule mk_eval_oracle_agrees
-    \\ simp [is_record_def]
+    fs [Case_def, markerTheory.Abbrev_def]
     \\ rpt strip_tac \\ fs []
+    \\ rveq \\ fs []
+    \\ TRY (drule_then irule mk_eval_oracle_agrees)
     \\ metis_tac []
   )
   \\ fs [s_rel_def]
@@ -1876,12 +1942,11 @@ QED
 Theorem oracle_semantics_prog:
   semantics_prog s1 env decs outcome /\
   outcome <> Fail /\
-  s1.eval_state = SOME (EvalDecs eds) /\
+  init_eval_state s1.eval_state /\
   s1.refs = [] /\
-  nsAll (K concrete_v) env.v /\
-  eds.env_id_counter = (0, 0, 1) ==>
-  semantics_prog (s1 with eval_state := mk_orac_st eds s1 env decs) env decs
-    outcome
+  nsAll (K concrete_v) env.v ==>
+  semantics_prog (s1 with eval_state := mk_orac_st c st0 s1 env decs)
+    env decs outcome
 Proof
   Cases_on `outcome` \\ rw []
   \\ fs [semantics_prog_def]
@@ -1893,16 +1958,147 @@ Proof
   )
   >- (
     drule evaluate_prog_with_clock_mk_orac_st
+    \\ simp []
+    \\ disch_then (qspecl_then [`st0`, `c`] mp_tac)
     \\ rw []
     \\ asm_exists_tac
     \\ imp_res_tac result_rel_IMP_cases \\ fs []
   )
 QED
 
-(* TODO: extra properties of mk_orac_st, in particular that the first
-   state satisfies the eds.compiler_state constraint *)
+Theorem mk_eval_oracle_init_wf:
+  s_rel eds s1 s2 /\
+  nsAll (K concrete_v) env.v /\
+  s1.eval_state = SOME (EvalDecs eds) /\
+  FST (FST ((orac_s s2.eval_state).oracle 0)) = 0 /\
+  ~ semantics_prog s1 env decs Fail
+  ==>
+  let (_, st, _) = mk_eval_oracle total_c st0 s2 env decs 0 in
+  (eds.compiler_state st \/ st = st0)
+Proof
+  rpt disch_tac
+  \\ Q.ISPECL_THEN [`st0`, `s2`, `0`, `env`, `decs`, `total_c`]
+    mp_tac mk_eval_oracle_def
+  \\ DEEP_INTRO_TAC whileTheory.OLEAST_INTRO
+  \\ rw []
+  \\ rpt (pairarg_tac \\ fs [])
+  \\ rveq \\ fs []
+  \\ drule_then (qspec_then `n` assume_tac) s_rel_clock2
+  \\ Cases_on `evaluate_decs (s1 with clock := n) env decs`
+  \\ drule_then drule (List.last (CONJUNCTS eval_simulation))
+  \\ disch_then (qspec_then `env` mp_tac)
+  \\ qpat_x_assum `~ _` mp_tac
+  \\ simp [semantics_prog_def, evaluate_prog_with_clock_def]
+  \\ disch_then (qspec_then `n` mp_tac)
+  \\ simp [elim_Case, env_rel_concrete_v]
+  \\ rw [s_rel_def]
+  \\ fs []
+  \\ rfs []
+QED
+
+Theorem mk_eval_oracle_wf:
+  s_rel eds s1 s2 /\
+  nsAll (K concrete_v) env.v /\
+  s1.eval_state = SOME (EvalDecs eds) /\
+  ~ semantics_prog s1 env decs Fail
+  ==>
+  let orac = mk_eval_oracle total_c st0 s2 env decs in
+  (!j. let next_st = FST (SND (orac (SUC j))) in
+    (?r. eds.compiler (orac j) = SOME r /\ FST r next_st) \/
+    next_st = FST (total_c (orac j)))
+Proof
+  rw []
+  \\ Q.ISPECL_THEN [`st0`, `s2`, `SUC j`, `env`, `decs`, `total_c`]
+    mp_tac mk_eval_oracle_def
+  \\ DEEP_INTRO_TAC whileTheory.OLEAST_INTRO
+  \\ rw []
+  \\ rpt (pairarg_tac \\ fs [])
+  \\ rveq \\ fs []
+  \\ Cases_on `evaluate_decs (s1 with clock := n) env decs`
+  \\ drule_then (qspec_then `n` assume_tac) s_rel_clock2
+  \\ drule_then drule (List.last (CONJUNCTS eval_simulation))
+  \\ disch_then (qspec_then `env` mp_tac)
+  \\ qpat_x_assum `~ _` mp_tac
+  \\ simp [semantics_prog_def, evaluate_prog_with_clock_def]
+  \\ disch_then (qspec_then `n` mp_tac)
+  \\ simp [elim_Case, env_rel_concrete_v]
+  \\ rw []
+  \\ qpat_x_assum `s_rel init_eds _ _` mp_tac
+  \\ rw [s_rel_def, recorded_orac_wf_def]
+  \\ fs []
+  \\ first_x_assum drule
+  \\ drule evaluate_compiler_preserved
+  \\ rw [] \\ fs []
+  \\ drule_then (drule_then (qspecl_then [`st0`, `total_c`] mp_tac))
+    mk_eval_oracle_agrees
+  \\ simp [orac_agrees_def]
+  \\ fs [ADD1]
+QED
+
+Theorem semantics_prog_Fail_unique:
+  semantics_prog st env prog Fail /\
+  semantics_prog st env prog outcome ==>
+  outcome = Fail
+Proof
+  rw [] \\ Cases_on `outcome` \\ fs [semantics_prog_def]
+  >- (
+    fs [PAIR_FST_SND_EQ]
+  )
+  >- (
+    rveq \\ fs []
+    \\ fs [evaluate_prog_with_clock_def]
+    \\ rpt (pairarg_tac \\ fs [])
+    \\ rveq \\ fs []
+    \\ dxrule_then drule evaluate_decs_clock_determ
+    \\ simp []
+    \\ every_case_tac
+    \\ fs []
+  )
+QED
+
+(* The constructed oracle is an infinite oracle where each state results from
+   the previous arguments to one of the compilers. To avoid partiality issues
+   though, there are two compilers provided, one of which must be total. *)
+Theorem mk_orac_st_orac_wf:
+  semantics_prog s1 env decs outcome /\
+  outcome <> Fail /\
+  init_eval_state s1.eval_state /\
+  s1.refs = [] /\
+  nsAll (K concrete_v) env.v ==>
+  ? orac_st.
+  mk_orac_st total_c st0 s1 env decs = SOME (EvalOracle orac_st) /\
+  let orac = orac_st.oracle in
+  ((?eds. s1.eval_state = SOME (EvalDecs eds) /\
+        eds.compiler_state (FST (SND (orac 0)))) \/
+    FST (SND (orac 0)) = st0) /\
+  (!j. let next_st = FST (SND (orac (SUC j))) in
+  (? eds r. s1.eval_state = SOME (EvalDecs eds) /\
+    eds.compiler (orac j) = SOME r /\ FST r next_st) \/
+  next_st = FST (total_c (orac j)))
+Proof
+  rw [mk_orac_st_def]
+  \\ every_case_tac \\ fs [init_eval_state_def]
+  \\ simp [mk_dummy_orac_def]
+  \\ qmatch_goalsub_abbrev_tac `_ with eval_state := SOME (EvalOracle orac_st)`
+  \\ `s_rel e s1 (s1 with <| eval_state := SOME (EvalOracle orac_st) |>)`
+  by ( unabbrev_all_tac
+    \\ simp [s_rel_def, state_component_equality, recorded_orac_wf_def] )
+  \\ `FST (orac_st.oracle 0) = (0, 0)` by ( fs [markerTheory.Abbrev_def] )
+  \\ simp [insert_oracle_def, shift_seq_def]
+  \\ drule_then (qsubterm_then `mk_eval_oracle _ _ _ _ _` mp_tac)
+        mk_eval_oracle_init_wf
+  \\ simp [UNCURRY]
+  \\ impl_keep_tac
+  >- (
+    strip_tac
+    \\ dxrule_then drule semantics_prog_Fail_unique
+    \\ simp []
+  )
+  \\ simp []
+  \\ drule_then (qsubterm_then `mk_eval_oracle _ _ _ _ _` mp_tac)
+        mk_eval_oracle_wf
+  \\ simp []
+QED
 
 val _ = export_theory ();
-
-
 
